consolidate bedrock2.Syntax.Basic; port examples

bedrock2/src/BasicC64Semantics.v
@@ -1,17 +1,16 @@
 Require Import Coq.ZArith.ZArith.
-Require Import bedrock2.Syntax bedrock2.BasicCSyntax bedrock2.Semantics.
+Require Import bedrock2.Syntax bedrock2.Syntax.Basic bedrock2.Semantics.
 Require coqutil.Datatypes.String coqutil.Map.SortedList coqutil.Map.SortedListString.
 Require Import coqutil.Word.Interface.
 Require coqutil.Word.Naive.
 
 Axiom StrictOrderWord : forall width word, @word.ok width word -> @SortedList.parameters.strict_order (@word.rep _ word) (@word.ltu _ word).
 
-Existing Instance Word.Naive.ok.
-Instance parameters : parameters :=
+Definition parameters : parameters :=
   let word := Word.Naive.word 64 eq_refl in
   let byte := Word.Naive.word 8 eq_refl in
   {|
-  syntax := StringNamesSyntax.make BasicCSyntax.StringNames_params;
+  syntax := Syntax.Basic.parameters;
   mem := SortedList.map (SortedList.parameters.Build_parameters word byte word.ltu) (StrictOrderWord _ _ _);
   locals := SortedListString.map _;
   env := SortedListString.map _;
@@ -19,7 +18,7 @@ Instance parameters : parameters :=
   ext_spec := fun _ _ _ _ _ => False;
 |}.
 
-Global Instance parameters_ok trace m0 act args :
+Instance ok (_ := parameters) trace m0 act args :
   Morphisms.Proper
     (Morphisms.respectful
        (Morphisms.pointwise_relation Interface.map.rep
